

Nathanson [88]: Prove that there does not exist a polynomial identity of the form:

$$(x_1^2 + x_2^2 + x_3^2)(y_1^2 + y_2^2 + y_3^2) = z_1^2 + z_2^2 + z_3^2$$

where z_1, z_2, z_3 are polynomials in x_1, x_2, y_1, y_2, y_3 with integral coefficients:

Proof: Setting $x_3 = y_3 = 0$ we obtain:

$$(x_1^2 + x_2^2)(y_1^2 + y_2^2) = z_1'^2 + z_2'^2 + z_3'^2$$

(with $x_3 = y_3 = 0$)

$$\Leftrightarrow x_1^2 y_1^2 + x_2^2 y_1^2 + x_1^2 y_2^2 + x_2^2 y_2^2 = z_1'^2 + z_2'^2 + z_3'^2$$

where z_1', z_2', z_3' are polynomials in x_1, x_2, y_1, y_2 only:

Any general polynomial in x_1, x_2, y_1, y_2 is of the form:

$$ax_1 y_1 + bx_1 y_2 + cx_2 y_1 + dx_2 y_2$$

$$a, b, c, d \in \mathbb{Z}$$

so let us assume that:

$$x_1^2 y_1^2 + x_2^2 y_1^2 + x_1^2 y_2^2 + x_2^2 y_2^2$$

$$= (ax_1y_1 + bx_1y_2 + cx_2y_1 + dx_2y_2)^2 \\ + (ex_1y_1 + fx_1y_2 + gx_2y_1 + hx_2y_2)^2 \\ + (ix_1y_1 + jx_1y_2 + kx_2y_1 + lx_2y_2)^2$$

comparing coefficients of x_1y_1 , x_1y_2 , x_2y_1 and x_2y_2 on both sides give us:

$$\begin{cases} a^2 + e^2 + i^2 = 1 & \text{①} \\ b^2 + f^2 + j^2 = 1 & \text{②} \\ c^2 + g^2 + k^2 = 1 & \text{③} \\ d^2 + h^2 + l^2 = 1 & \text{④} \end{cases}$$

Next coefficients of cross terms like $x_1^2 y_1 y_2$, $x_2^2 y_1 y_2$ etc should be zero on the RHS because no such terms appear on the LHS: ~~the~~
 ~~give~~

This gives us the equations:

$$\begin{cases} ab + ef + ij = 0 & \text{--- } ①' \\ ac + eg + ik = 0 & \text{--- } ②' \\ ad + eh + il = 0 & \text{--- } ③' \\ bc + fg + jk = 0 & \text{--- } ④' \\ bd + fh + jl = 0 & \text{--- } ⑤' \\ cd + gh + kl = 0 & \text{--- } ⑥' \end{cases}$$

$$① \Rightarrow a^2 + e^2 + i^2 = 1$$

where $a, e, i \in \mathbb{Z}$.

w.l.o.g assume $a = \pm 1, e = i = 0$.

With $e = i = 0$ and $a = \pm 1$, $①'$ implies $b = 0$.

$$\text{Now } ② \Rightarrow f^2 + j^2 = 1.$$

w.l.o.g assume $f = \pm 1$ and $j = 0$.

$$④' \Rightarrow g = 0$$

$$⑤' \Rightarrow h = 0.$$

$$\textcircled{3} \Leftrightarrow c^2 + g^2 + k^2 = 1$$

$$\Rightarrow c^2 + k^2 = 1 \quad (\because g = 0)$$

~~at a g assume~~ But,

$$ac + eg + ik = 0$$

$$\Leftrightarrow (\pm 1)c + 0 \cdot 0 + 0 \cdot k = 0$$

$$\Rightarrow c = 0.$$

$$\text{so } \textcircled{3} \Rightarrow c^2 + k^2 = 1$$

$$\Leftrightarrow k = \pm 1.$$

$$\textcircled{4}' \Rightarrow j = 0$$

$$\textcircled{6}' \Rightarrow l = 0$$

$$\textcircled{3}' \Rightarrow ad + 0 + 0 = 0$$

$$\Rightarrow d = 0$$

$$\text{so } d^2 + h^2 + l^2 = 0^2 + 0^2 + 0^2$$

$$\text{But } \textcircled{4} \Rightarrow d^2 + h^2 + l^2 = 1$$

A contradiction.